\documentclass[]{article}
\usepackage{amsmath}
\usepackage{amsfonts}
\usepackage[margin=1.0in]{geometry}
%opening
\author{}

\begin{document}
\textbf{Change of basis}
\vspace{1pc}

There are 2 standard ways to record a change of basis in $\mathbb{R}^n$ from an old basis $v_i$ to a new one $w_i$:
\begin{enumerate}
\item{The linear map $L:\mathbb{R}^n\rightarrow\mathbb{R}^n$ that sends each $v_i$ to $w_i$, and its matrix in the $v_i$ basis:
\[ P=[L]_{v_i}=\left[\left(\underset{\text{ in v basis}}{w_1}\right)\text{ }\left(\underset{\text{ in v basis}}{w_2}\right) ...\right] \]

So $L(v_i)=w_i$
}
\item{A matrix that converts column vectors expressed in the $v_i$ basis into their expression in the $w_i$ basis:
\[B=\left[\left(\underset{\text{ in w basis}}{v_1}\right)\text{ }\left(\underset{\text{ in w basis}}{v_2}\right) ...\right] \]

So $B\cdot \left[a\right]_{v_i}=\left[a\right]_{w_i}$
}
\end{enumerate}

Actually, $B=P^{-1}$ and $P=B^{-1}$, so while $B$ converts expressions in the old basis into their expressions in the new, $P$ converts the new to the old.

\begin{center}
\begin{tabular} {l l l l}
things that can be represented & by matrices (in basis $v_i$) & change of basis formulas & type of tensor\\
\hline
linear maps $L:\mathbb{R}^n\rightarrow\mathbb{R}^n$ & $a_{ij}=(L(v_j))_i$ & $M'=BMB^{-1}=P^{-1}MP$ & $\mathbb{R}^n\otimes \mathbb{R}^{n*}$ \\
bilinear forms $L:\mathbb{R}^n\times\mathbb{R}^n\rightarrow \mathbb{R}$ & $a_{ij}=L(v_i,v_j) $  & $M'=(B^{-1})^{T}MB^{-1}=P^{T}MP$ & $\mathbb{R}^{n*}\otimes\mathbb{R}^{n*}$\\
bilinear forms $L:\mathbb{R}^{n*}\times\mathbb{R}^{n*}\rightarrow \mathbb{R}$ & $a_{ij}=L(v_i^{*},v_j^{*})$ & $M'=BMB^{T}=P^{-1}M(P^{-1})^{T}$ & $\mathbb{R}^n\otimes\mathbb{R}^n$\\
\end{tabular}
\end{center}

\begin{itemize}
\item{With the matrix $M$ of a linear map $L$ with respect to $v_i$, $M\cdot \left[a \text{ in }v_i\text{ basis}\right]=\left[L(a) \text{ in }v_i\text{ basis}\right]$, and
\[BMB^{-1}\left[a \text{ in new }w_i\text{ basis}\right]=\left[L(a) \text{ in new }w_i\text{ basis}\right]\]
}
\item{With the matrix $M$ of a bilinear form $L$ with respect to $v_i$, $L(a,b)=\left[a \text{ in }v_i\text{ basis}\right]^{T}M\left[b\text{ in }v_i\text{ basis}\right]$, and also
\[L(a,b)=\left[a \text{ in new }w_i\text{ basis}\right]^{T}(B^{-1})^{T}MB^{-1}\left[b\text{ in new }w_i\text{ basis}\right] \]
}
\end{itemize}
\end{document}
